1. $y = u^3, u = x^2+1$
	1. $\frac{dy}{dx} = ?$
	2. $\frac{dy}{dx} = (x^2 +1)^3 \Rightarrow 3(x^2+1)^2 \times 2x$
	3. Or you can use chain rule
2. $y = u^2, u=sin(x)cos(x)$
	1. $y' = (sin(x)cos(x))^2 \Rightarrow 2(sin(x)cos(x)) \times cos^2(x) - sin^2(x)$
	2. $y' = sin(2x)cos(2x)$
3. $f(t) = \frac{1}{\frac{1}{1+\frac{1}{t}}  +1}$
	1. $f(t) = [(1+\frac{1}{t})^{-1} +1]^{-1}$
	2. Using the chain rule or 
	3. $f'(t) = -1[(1+t^{-1})^{-1}+1]^{-2} \times [-1(1+t^{-1})^{-2}(-\frac{1}{t^2})]$
	4. ...
	5. $f'(t) = -\frac{1}{(2t+1)^2}$
4. Find the slope at $(1,-2)$ for $y^4 +3y -4x^3 = 5x+1$.
	1. [[Implicit Differentiation]]
	2. $4y^3(\frac{dy}{dx}) + 3(\frac{dy}{dx}) -12x^2 = 5$
	3. $(\frac{dy}{dx})(4y^3 +3) = 5+12x^2$
	4. $\frac{dy}{dx} = \frac{12x^2+5}{4y^3+3}$
	5. $\frac{dy}{dx} = \frac{12(1)^2 +5}{4(-8)+3}$
	6. $\frac{dy}{dx} = -\frac{17}{29}$
5. 