#Lecture
- $\lim_{x\to9}(\frac{x-9}{\sqrt{x}-3})$ $\Rightarrow$ $\lim_{x\to9}(\frac{(\sqrt{x}-3)(\sqrt{x}+3)}{\sqrt{x}-3})$ $\Rightarrow$ $\lim_{x\to9}(\sqrt{x}-3)$ $\Rightarrow$ $6$
- Format: $\frac{a\times-a}{a}$
- [[Definition]] of [[Limits]]: 
  $\lim_{x\to a} f(x) = L \Longrightarrow$ 
  for every $\epsilon > 0,$ there exists $\delta > 0,$ such that
  if $0 < |x-a| < \delta$, then $|f(x)-L| < \epsilon$
- $\lim_{x\to4}(\frac{1}{2}(3x-1) = \frac{11}{2}$ (planting everything into the definition:)
  $|\frac{1}{2}(3x-1) - \frac{11}{2}| < \epsilon$
  $|(3x-1) - 11| <2 \epsilon$
  $|x-4| < \frac{2}{3} \epsilon$
  $\delta = \frac{2}{3} \epsilon$
- **How do you decipher [[Mathematical Definitions]]?**
- $\lim_{x\to2}\sqrt{x-2} \Rightarrow$ coming from $> 2$ is approaches $0$, and coming from $<2$ it gives us an imaginary number. So: $\lim_{x\to2^+}\sqrt{x-2} \Rightarrow 0$ 
  This is called a *[[One Sided Limit]]*
- 