#Lecture 
[[Derivative of Inverse Functions]]
1. $y=7x-55$
	1. Inverse: $x=\frac{y+55}{7}$
	2. $\frac{dy}{dx} = 7$
	3. $\frac{dx}{dy} = \frac{1}{7}$
2. $y = 1 + \frac{1}{x}$
	1. $y = 1 + x^{-1} \Rightarrow x = \frac{1}{y-1}$
	2. $\frac{dy}{dx} = -x^{-2}$
	3. $\frac{dx}{dy} = \frac{1}{(y-1)^2}$
3. $y = x^3$
	1. $x = \sqrt[3]{y}$
	2. $\frac{dy}{dx} = 3x^2$
	3. $\frac{dx}{dy} = \frac{1}{3}y^{-\frac{2}{3}}$
4. **Rule:** $f^{-1}\\'(x) = \frac{1}{f'(f^{-1}(x))}$
	1. $y = 7x-55$
		1. $f'(x) = 7$
		2. $f^{-1}(x) = \frac{x+55}{7}$
		3. $f^{-1}\\'(x) = \frac{1}{7}$
	2. $f(x) = x^3$
		1. $f'(x) = 3x^2$
		2. $f^{-1}(x) = x^{\frac{1}{3}}$
		3. $f^{-1}\\'(x) = \frac{1}{3(x^{\frac{1}{3}})^2} \Rightarrow \frac{1}{3}x^{-\frac{2}{3}}$
	3. $$f(x) = \sqrt{2x+3} \Rightarrow (2x+3)^{\frac{1}{2}}$$
		1. $$f'(x) = \frac{1}{\sqrt{2x+3}}$$
		2. $$f^{-1}(x) = \frac{x^2-3}{2}$$
		3. $$f^{-1}\\'(x) = \frac{1}{\frac{1}{\sqrt{2(\frac{x^2-3}{2})+3}}} \Rightarrow x$$
	4. Question 2: $$f(x) = 4-x^2, x\geq0$$
		1. $$f^{-1}(x) = \sqrt{4-x}$$
		2. $$f'(x) = -2x$$
		3. $$f^{-1}\\'(x) = -\frac{1}{2\sqrt{4-x}}$$
	5. $$f(x) = sin(x)$$
		1. $$f'(x) = cos(x)$$
		2. $$f^{-1}(x) = sin^{-1}(x)$$
		3. $$f^{-1}\\'(x) = \frac{1}{\sqrt{1-x^2}}$$
			1. $y=sin^{-1}(x)$
			2. $sin(y) = x$
			3. $(cos(y))\frac{dy}{dx} = 1$
			4. $\frac{dy}{dx} = \frac{1}{cos(x)}$
			5. $\to sin^2(x) + cos^2(x) = 1$
			6. $x^2 + cos^2(x) = 1$
			7. $cos(x) = \sqrt{1-x^2}$
			8. $\Rightarrow \frac{dy}{dx} = \frac{1}{cos(y)} = \frac{1}{\sqrt{1-x^2}}$
5. Wednesday $5:30$ Research Proposal
6. 